---
title:      Exercise 4.4-3
clrs:       [4, 4]
published:  2012-08-28 21:10
redirect_from:
  - /E04.04-03/
---

>Use a recursion tree to determine a good asymptotic upper bound on the recurrence $$T(n) = 4T(n/2 + 2) + n$$. Use the substitution method to verify your answer.

Rate of increase in number of subproblems in each recursion = 4
Rate of decrease in subproblem size = 2 with additional 2 inputs

Hence in each level of the tree, there are $$4^i$$ nodes each of cost $$c(n/2^i + 2)$$ at depth $$i = 0, 1, 2, \dots, \lg n$$.

Hence, total cost of the tree is:

$$\begin {align}
T(n) & = \sum_{i = 0}^{\lg n} 4^i \cdot c\left(\frac n {2^i} + 2\right) \\
     & = \sum_{i = 0}^{\lg n} 4^i \cdot c\frac n {2^i} + \sum_{i = 0}^{\lg n} 4^i \cdot c \cdot 2 \\
     & = cn \sum_{i = 0}^{\lg n} \frac {4^i} {2^i} + 2c \sum_{i = 0}^{\lg n} 4^i \\
     & = cn \sum_{i = 0}^{\lg n} 2^i + 2c \sum_{i = 0}^{\lg n} 4^i \\
     & = cn \frac {2^{\lg n + 1} - 1} {2 - 1} + 2c \frac {4^{\lg n + 1} - 1} {4 - 1} \\
     & = cn (2^{\lg n + 1} - 1) + \frac {2c} 3 (4^{\lg n + 1} - 1) \\
     & = cn (2 \cdot 2^{\lg n} - 1) + \frac {2c} 3 (4 \cdot 4^{\lg n} - 1) \\
     & = cn (2 \cdot n - 1) + \frac {2c} 3 (4 \cdot n^2 - 1) \\
     & = 2cn^2 - 2n + \frac {8cn^2} 3 - \frac {2c} 3 \\
     & = O(n^2)
\end {align}$$

Now we have to show that our guess $$T(n) = O(n^2)$$ holds using the substitution method. Let's refine our guess to $$T(n) \le d(n^2 - bn)$$ for positive constants $$b$$ and $$d$$.

$$\begin {align}
T(n) & = 4T(n/2 + 2) + n \\
     & \le 4d((n/2 + 2)^2 - b(n/2 + 2)) + n \\
     & = 4d(n^2/4 + 2n + 4 - bn/2 - 2b) + n \\
     & = dn^2 + 8dn + 16d - 2dbn - 8db + n \\
     & = dn^2 - dbn + 8dn + 16d - dbn - 8db + n \\
     & = d(n^2 - bn) - (db - 8d - 1)n - (b - 2)8d \\
     & \le d(n^2 - bn)
\end {align}$$

The last step holds as long as $$db - 8d - 1 \ge 0$$.